FokkerChallenge/BLC/Blc.lean
@@ -7,11 +7,11 @@ def main : IO Unit := do
   let terms := terms.filter (fun t => !Cslib.LambdaCalculus.LocallyNameless.Untyped.Term.every_bvar_used t)
   let terms := terms.filter (fun t => !Cslib.LambdaCalculus.LocallyNameless.Untyped.Term.only_one_var_used t)
   let terms := terms.filter (fun t => !Cslib.LambdaCalculus.LocallyNameless.Untyped.Term.no_duplicate t)
-  let terms := terms.filter (fun t => !Cslib.LambdaCalculus.LocallyNameless.Untyped.Term.isNamedOfXY t)
   let terms := terms.filter (fun t => !Cslib.LambdaCalculus.LocallyNameless.Untyped.Term.tailOk t)
   let terms := terms.filter (fun t => !Cslib.LambdaCalculus.LocallyNameless.Untyped.Term.rigid t)
   let terms := terms.filter (fun t => !Cslib.LambdaCalculus.LocallyNameless.Untyped.Term.argOk t)
   let terms := terms.filter (fun t => !Cslib.LambdaCalculus.LocallyNameless.Untyped.Term.properClosedNoParens t)
+  let terms := terms.filter (fun t => !Cslib.LambdaCalculus.LocallyNameless.Untyped.Term.closedNodeTwoVars t)
 
   let terms := terms.filter (fun t => t ∉ Cslib.LambdaCalculus.LocallyNameless.Untyped.Term.fokkerUndecidedTerms)
   let terms := terms.filter (fun t => t ∉ Cslib.LambdaCalculus.LocallyNameless.Untyped.Term.fokkerUpdatedOpenCerts.map Prod.fst)
